#################################################################
###  Generated with the experimental alpha version of the TTL exporter of WebVOWL (version 1.1.7)  http://visualdataweb.de/webvowl/   ###
#################################################################

@prefix : 		<https://w3id.org/hmo#> .
@prefix rdf: 		<http://www.w3.org/1999/02/22-rdf-syntax-ns#> .
@prefix rdfs: 		<http://www.w3.org/2000/01/rdf-schema#> .
@prefix owl: 		<http://www.w3.org/2002/07/owl#> .
@prefix xsd: 		<http://www.w3.org/2001/XMLSchema#> .
@prefix dc: 		<http://purl.org/dc/elements/1.1/> .
@prefix xml: 		<http://www.w3.org/XML/1998/namespace> .
@prefix wot: 		<http://xmlns.com/wot/0.1/> .
@prefix vs: 		<http://www.w3.org/2003/06/sw-vocab-status/ns#> .
@prefix foaf: 		<http://xmlns.com/foaf/0.1/> .
@prefix : 		<https://w3id.org/hmo#> .
@base 			<https://w3id.org/hmo#> .

<https://w3id.org/hmo#> rdf:type owl:Ontology ;
                        dc:title "Historic Masonry Ontology"@en; 
                        dc:description "Ontology to represent the historic masonry material"@en; 
                        owl:versionInfo "0.1"@en;
                        dc:creator "Maria Laura Leonardi, Stefano Cursi, Elena Gigliarelli, Jos√© Granja, Daniel Oliveira, Miguel Azenha." . 
#################################################################

###  Property Definitions (Number of Property) 48 ###
#  --------------------------- Property 0------------------------- 
:MQIWallLeavesConnectionsInPlane rdf:type owl:DatatypeProperty ;
                                 rdfs:comment "Defines the adequacy of connections of the adjacent leaves in a wall, in the context of in plane loading." ;
                                 rdfs:label "MQIWallLeavesConnectionsInPlane"@IRI-based; 
                                 rdfs:label "MQI-In Plane-Wall Leaves Connection"@en; 
                                 rdfs:domain :MasonryQualityIndex;
                                 rdfs:range xsd:float . 
#  --------------------------- Property 1------------------------- 
:areInterfaceElementsOf rdf:type owl:ObjectProperty; 
                        owl:inverseOf :hasInterfaceElements ;
                        rdfs:comment "Defines the relationship between joints and units in a pattern." ;
                        rdfs:label "areInterfaceElementsOf"@IRI-based; 
                        rdfs:label "are interface elements of"@en; 
                        rdfs:domain :Joints;
                        rdfs:range :Units . 
#  --------------------------- Property 2------------------------- 
:MQIUnitsPropertiesVert rdf:type owl:DatatypeProperty ;
                        rdfs:comment "Defines the adequacy of mechanical properties of the units, in the context of vertical loading." ;
                        rdfs:label "MQIUnitsPropertiesVert"@IRI-based; 
                        rdfs:label "MQI-Vertical-Units Properties"@en; 
                        rdfs:domain :MasonryQualityIndex;
                        rdfs:range xsd:float . 
#  --------------------------- Property 3------------------------- 
:MQIUnitsPropertiesInPlane rdf:type owl:DatatypeProperty ;
                           rdfs:comment "Defines the adequacy of mechanical properties of the units, in the context of in plane loading." ;
                           rdfs:label "MQIUnitsPropertiesInPlane"@IRI-based; 
                           rdfs:label "MQI-In Plane-Units Properties"@en; 
                           rdfs:domain :MasonryQualityIndex;
                           rdfs:range xsd:float . 
#  --------------------------- Property 4------------------------- 
:hasSparsePatternEntities rdf:type owl:ObjectProperty; 
                          owl:inverseOf :areSparsePatternEntitiesOf ;
                          rdfs:comment "Determines which pattern entities are sparse in a pattern." ;
                          rdfs:label "hasSparsePatternEntities"@IRI-based; 
                          rdfs:label "has sparse pattern entities"@en; 
                          rdfs:domain :Pattern;
                          rdfs:range :PatternEntities . 
#  --------------------------- Property 5------------------------- 
<https://saref.etsi.org/core/isMeasuredIn> rdf:type owl:DatatypeProperty ;
                                           rdfs:label "isMeasuredIn"@IRI-based; 
                                           rdfs:range rdfs:Literal . 
#  --------------------------- Property 6------------------------- 
:MQIVerticalJointsInPlane rdf:type owl:DatatypeProperty ;
                          rdfs:comment "Defines the adequacy of In plane joints (based on staggered properties), in the context of in plane loading." ;
                          rdfs:label "MQIVerticalJointsInPlane"@IRI-based; 
                          rdfs:label "MQI-In Plane-Vertical Joints"@en; 
                          rdfs:domain :MasonryQualityIndex;
                          rdfs:range xsd:float . 
#  --------------------------- Property 7------------------------- 
:isHomogenisedMechanicalPropertyOf rdf:type owl:ObjectProperty; 
                                   owl:inverseOf :hasHomogenisedMechanicalProperty ;
                                   rdfs:comment "Defines the relationship between an homogenised mechanical property and a masonry wall." ;
                                   rdfs:label "isHomogenisedMechanicalPropertyOf"@IRI-based; 
                                   rdfs:label "is homogenised mechanical property of"@en; 
                                   rdfs:domain :HomogenisedMechanicalProperty;
                                   rdfs:range :RepresentativeVolumeElement . 
#  --------------------------- Property 8------------------------- 
:MQIUnitsShapeInPlane rdf:type owl:DatatypeProperty ;
                      rdfs:comment "Defines the adequacy of the units shape, in the context of in plane loading." ;
                      rdfs:label "MQIUnitsShapeInPlane"@IRI-based; 
                      rdfs:label "MQI-In Plane-Units Shape"@en; 
                      rdfs:domain :MasonryQualityIndex;
                      rdfs:range xsd:float . 
#  --------------------------- Property 9------------------------- 
:isLocatedIn rdf:type owl:ObjectProperty ;
             rdfs:comment "Defines the Masonry Layer where a pattern is located." ;
             rdfs:label "isLocatedIn"@IRI-based; 
             rdfs:label "is located of"@en; 
             rdfs:domain :Pattern;
             rdfs:range :MasonryLayer . 
#  --------------------------- Property 10------------------------- 
:isPatternOf rdf:type owl:ObjectProperty; 
             owl:inverseOf :hasPattern ;
             rdfs:comment "Used to define when one or more patterns are present in a Representative Volume Element." ;
             rdfs:label "isPatternOf"@IRI-based; 
             rdfs:label "is pattern of"@en; 
             rdfs:domain :Pattern;
             rdfs:range :RepresentativeVolumeElement . 
#  --------------------------- Property 11------------------------- 
:MQIUnitsDimensionsVert rdf:type owl:DatatypeProperty ;
                        rdfs:comment "Defines the adequacy of units size, in the context of vertical loading." ;
                        rdfs:label "MQIUnitsDimensionsVert"@IRI-based; 
                        rdfs:label "MQI-Vertical-Units Dimensions"@en; 
                        rdfs:domain :MasonryQualityIndex;
                        rdfs:range xsd:float . 
#  --------------------------- Property 12------------------------- 
:MQIMortarQualityInPlane rdf:type owl:DatatypeProperty ;
                         rdfs:comment "Defines the adequacy of the mortar, in the context of in plane loading." ;
                         rdfs:label "MQIMortarQualityInPlane"@IRI-based; 
                         rdfs:label "MQI-In Plane-Mortar Quality"@en; 
                         rdfs:domain :MasonryQualityIndex;
                         rdfs:range xsd:float . 
#  --------------------------- Property 13------------------------- 
:MQIMortarQualityOutOfPlane rdf:type owl:DatatypeProperty ;
                            rdfs:comment "Defines the adequacy of the mortar, in the context of out of plane loading." ;
                            rdfs:label "MQIMortarQualityOutOfPlane"@IRI-based; 
                            rdfs:label "MQI-Out Of Plane-Mortar Quality"@en; 
                            rdfs:domain :MasonryQualityIndex;
                            rdfs:range xsd:float . 
#  --------------------------- Property 14------------------------- 
:MQIVerticalJointsOutOfPlane rdf:type owl:DatatypeProperty ;
                             rdfs:comment "Defines the adequacy of Out of plane joints (based on staggered properties), in the context of out of plane loading." ;
                             rdfs:label "MQIVerticalJointsOutOfPlane"@IRI-based; 
                             rdfs:label "MQI-Out Of Plane-Vertical Joints"@en; 
                             rdfs:domain :MasonryQualityIndex;
                             rdfs:range xsd:float . 
#  --------------------------- Property 15------------------------- 
:MQIUnitsDimensionsInPlane rdf:type owl:DatatypeProperty ;
                           rdfs:comment "Defines the adequacy of units size, in the context of in plane loading." ;
                           rdfs:label "MQIUnitsDimensionsInPlane"@IRI-based; 
                           rdfs:label "MQI-In Plane-Units Dimensions"@en; 
                           rdfs:domain :MasonryQualityIndex;
                           rdfs:range xsd:float . 
#  --------------------------- Property 16------------------------- 
:areSparsePatternEntitiesOf rdf:type owl:ObjectProperty; 
                            owl:inverseOf :hasSparsePatternEntities ;
                            rdfs:comment "It determines when a pattern entity is'sparse'in a pattern, i.e. when it has a distribution of less than 50 per cent in the pattern. " ;
                            rdfs:label "areSparsePatternEntitiesOf"@IRI-based; 
                            rdfs:label "are sparse pattern entities of"@en; 
                            rdfs:domain :PatternEntities;
                            rdfs:range :Pattern . 
#  --------------------------- Property 17------------------------- 
:MQIVerticalJointsVert rdf:type owl:DatatypeProperty ;
                       rdfs:comment "Defines the adequacy of vertical joints (based on staggered properties), in the context of vertical loading." ;
                       rdfs:label "MQIVerticalJointsVert"@IRI-based; 
                       rdfs:label "MQI-Vertical-Vertical Joints"@en; 
                       rdfs:domain :MasonryQualityIndex;
                       rdfs:range xsd:float . 
#  --------------------------- Property 18------------------------- 
:MQIHorizontalJointsOutOfPlane rdf:type owl:DatatypeProperty ;
                               rdfs:comment "Defines the adequacy of horizontal joints (based on level of horizontality/continuity), in the context of out of plane loading." ;
                               rdfs:label "MQIHorizontalJointsOutOfPlane"@IRI-based; 
                               rdfs:label "MQI-Out Of Plane-Horizontal Joints"@en; 
                               rdfs:domain :MasonryQualityIndex;
                               rdfs:range xsd:float . 
#  --------------------------- Property 19------------------------- 
:MQIUnitsShapeVert rdf:type owl:DatatypeProperty ;
                   rdfs:comment "Defines the adequacy of the units shape, in the context of vertical loading." ;
                   rdfs:label "MQIUnitsShapeVert"@IRI-based; 
                   rdfs:label "MQI-Vertical-Units Shape"@en; 
                   rdfs:domain :MasonryQualityIndex;
                   rdfs:range xsd:float . 
#  --------------------------- Property 20------------------------- 
:MQITotalVertical rdf:type owl:DatatypeProperty ;
                  rdfs:comment "Defines the total value of MQI for vertical loads" ;
                  rdfs:label "MQITotalVertical"@IRI-based; 
                  rdfs:label "Masonry Quality Index total value for vertical loads"@en; 
                  rdfs:domain :MasonryQualityIndex;
                  rdfs:range xsd:float . 
#  --------------------------- Property 21------------------------- 
:jointsThickness rdf:type owl:DatatypeProperty ;
                 rdfs:comment "Defines the thickness of the joints. " ;
                 rdfs:label "jointsThickness"@IRI-based; 
                 rdfs:label "Joint Thickness"@en; 
                 rdfs:domain :Units;
                 rdfs:range xsd:float . 
#  --------------------------- Property 22------------------------- 
:hasRepresentativeVolumeElement rdf:type owl:ObjectProperty ;
                                rdfs:comment "Defines the representative volume element of a wall" ;
                                rdfs:label "hasRepresentativeVolumeElement"@IRI-based; 
                                rdfs:label "has representative volume element"@en; 
                                rdfs:domain :MasonryElement;
                                rdfs:range :RepresentativeVolumeElement . 
#  --------------------------- Property 23------------------------- 
:hasInterfaceElements rdf:type owl:ObjectProperty; 
                      owl:inverseOf :areInterfaceElementsOf ;
                      rdfs:comment "Defines the relationship between units and joints in a pattern." ;
                      rdfs:label "hasInterfaceElements"@IRI-based; 
                      rdfs:label "has interface elements"@en; 
                      rdfs:domain :Units;
                      rdfs:range :Joints . 
#  --------------------------- Property 24------------------------- 
:MQITotalInPlane rdf:type owl:DatatypeProperty ;
                 rdfs:comment "Defines the total value of MQI for in plane loads" ;
                 rdfs:label "MQITotalInPlane"@IRI-based; 
                 rdfs:label "Masonry Quality Index total value for in plane loads"@en; 
                 rdfs:domain :MasonryQualityIndex;
                 rdfs:range xsd:float . 
#  --------------------------- Property 25------------------------- 
:unitsLengthMaximumValue rdf:type owl:DatatypeProperty ;
                         rdfs:comment "Defines the maximum value of the length of the units in the pattern. " ;
                         rdfs:label "unitsLengthMaximumValue"@IRI-based; 
                         rdfs:label "Units Length Has Maximum Value"@en; 
                         rdfs:domain :Units;
                         rdfs:range xsd:float . 
#  --------------------------- Property 26------------------------- 
:areDominantPatternEntitiesOf rdf:type owl:ObjectProperty; 
                              owl:inverseOf :hasDominantPatternEntities ;
                              rdfs:comment "It determines when a pattern entity is 'dominant' in a pattern, i.e. when it has a distribution greater than 50% in the pattern." ;
                              rdfs:label "areDominantPatternEntitiesOf"@IRI-based; 
                              rdfs:label "are dominant pattern entities of"@en; 
                              rdfs:domain :PatternEntities;
                              rdfs:range :Pattern . 
#  --------------------------- Property 27------------------------- 
:MQIWallLeavesConnectionsVert rdf:type owl:DatatypeProperty ;
                              rdfs:comment "Defines the adequacy of connections of the adjacent leaves in a wall, in the context of vertical loading." ;
                              rdfs:label "MQIWallLeavesConnectionsVert"@IRI-based; 
                              rdfs:label "MQI-Vertical-Wall Leaves Connection"@en; 
                              rdfs:domain :MasonryQualityIndex;
                              rdfs:range xsd:float . 
#  --------------------------- Property 28------------------------- 
:MQIHorizontalJointsInPlane rdf:type owl:DatatypeProperty ;
                            rdfs:comment "Defines the adequacy of horizontal joints (based on level of horizontality/continuity), in the context of in plane loading." ;
                            rdfs:label "MQIHorizontalJointsInPlane"@IRI-based; 
                            rdfs:label "MQI-In Plane-Horizontal Joints"@en; 
                            rdfs:domain :MasonryQualityIndex;
                            rdfs:range xsd:float . 
#  --------------------------- Property 29------------------------- 
:MQIUnitsDimensionsOutOfPlane rdf:type owl:DatatypeProperty ;
                              rdfs:comment "Defines the adequacy of units size, in the context of out of plane loading." ;
                              rdfs:label "MQIUnitsDimensionsOutOfPlane"@IRI-based; 
                              rdfs:label "MQI-Out Of Plane-Units Dimensions"@en; 
                              rdfs:domain :MasonryQualityIndex;
                              rdfs:range xsd:float . 
#  --------------------------- Property 30------------------------- 
#<https://saref.etsi.org/core/hasValue> rdf:type owl:DatatypeProperty ;
#                                       rdfs:label "hasValue"@IRI-based; 
#                                       rdfs:range rdfs:Literal . 
#  --------------------------- Property 31------------------------- 
:MQITotalOutOfPlane rdf:type owl:DatatypeProperty ;
                    rdfs:comment "Defines the total value of MQI for out of plane loads" ;
                    rdfs:label "MQITotalOutOfPlane"@IRI-based; 
                    rdfs:label "Masonry Quality Index total value for out of plane loads"@en; 
                    rdfs:domain :MasonryQualityIndex;
                    rdfs:range xsd:float . 
#  --------------------------- Property 32------------------------- 
:hasPattern rdf:type owl:ObjectProperty; 
            owl:inverseOf :isPatternOf ;
            rdfs:comment "Defines the relationship between a representative volume elements and a pattern." ;
            rdfs:label "hasPattern"@IRI-based; 
            rdfs:label "has pattern"@en; 
            rdfs:domain :RepresentativeVolumeElement;
            rdfs:range :Pattern . 
#  --------------------------- Property 33------------------------- 
:unitsHeightHasMaximumValue rdf:type owl:DatatypeProperty ;
                            rdfs:comment "Defines the maximum value of the height of the units in the pattern. " ;
                            rdfs:label "unitsHeightHasMaximumValue"@IRI-based; 
                            rdfs:label "Units Height Has Maximum Value"@en; 
                            rdfs:domain :Units;
                            rdfs:range xsd:float . 
#  --------------------------- Property 34------------------------- 
:unitsLengthHasMinimumValue rdf:type owl:DatatypeProperty ;
                            rdfs:comment "Defines the minimum value of the length of the units in the pattern. " ;
                            rdfs:label "unitsLengthHasMinimumValue"@IRI-based; 
                            rdfs:label "Units Length Has Minimum Value"@en; 
                            rdfs:domain :Units;
                            rdfs:range xsd:float . 
#  --------------------------- Property 35------------------------- 
:MQIWallLeavesConnectionsOutOfPlane rdf:type owl:DatatypeProperty ;
                                    rdfs:comment "Defines the adequacy of connections of the adjacent leaves in a wall, in the context of out of plane loading." ;
                                    rdfs:label "MQIWallLeavesConnectionsOutOfPlane"@IRI-based; 
                                    rdfs:label "MQI-Out Of Plane-Wall Leaves Connection"@en; 
                                    rdfs:domain :MasonryQualityIndex;
                                    rdfs:range xsd:float . 
#  --------------------------- Property 36------------------------- 
:unitsHeigthHasMinimumValue rdf:type owl:DatatypeProperty ;
                            rdfs:comment "Defines the minimum value of the height of the units in the pattern. " ;
                            rdfs:label "unitsHeigthHasMinimumValue"@IRI-based; 
                            rdfs:label "Units Height Has Minimum Value"@en; 
                            rdfs:domain :Units;
                            rdfs:range xsd:float . 
#  --------------------------- Property 37------------------------- 
:MQIUnitsPropertiesOutOfPlane rdf:type owl:DatatypeProperty ;
                              rdfs:comment "Defines the adequacy of mechanical properties of the units, in the context of out of plane loading." ;
                              rdfs:label "MQIUnitsPropertiesOutOfPlane"@IRI-based; 
                              rdfs:label "MQI-Out Of Plane-Units Properties"@en; 
                              rdfs:domain :MasonryQualityIndex;
                              rdfs:range xsd:float . 
#  --------------------------- Property 38------------------------- 
:bricksHaveVolumePercentage rdf:type owl:DatatypeProperty ;
                            rdfs:comment "In hollow bricks, it defines the percentage of volume, espressed in decimal (eg: 0.4 for 40%). " ;
                            rdfs:label "bricksHaveVolumePercentage"@IRI-based; 
                            rdfs:label "Bricks have volume percentage"@en; 
                            rdfs:domain :Units;
                            rdfs:range xsd:decimal . 
#  --------------------------- Property 39------------------------- 
:MQIUnitsShapeOutOfPlane rdf:type owl:DatatypeProperty ;
                         rdfs:comment "Defines the adequacy of the units shape, in the context of out of plane loading." ;
                         rdfs:label "MQIUnitsShapeOutOfPlane"@IRI-based; 
                         rdfs:label "MQI-Out Of Plane-Units Shape"@en; 
                         rdfs:domain :MasonryQualityIndex;
                         rdfs:range xsd:float . 
#  --------------------------- Property 40------------------------- 
:hasHomogenisedMechanicalProperty rdf:type owl:ObjectProperty; 
                                  owl:inverseOf :isHomogenisedMechanicalPropertyOf ;
                                  rdfs:comment "Defines the relationship between a representative volume element and an homogenised mechanical property." ;
                                  rdfs:label "hasHomogenisedMechanicalProperty"@IRI-based; 
                                  rdfs:label "has homogenised mechanical property"@en; 
                                  rdfs:domain :RepresentativeVolumeElement;
                                  rdfs:range :HomogenisedMechanicalProperty . 
#  --------------------------- Property 41------------------------- 
:hasDominantPatternEntities rdf:type owl:ObjectProperty; 
                            owl:inverseOf :areDominantPatternEntitiesOf ;
                            rdfs:comment "Determines which pattern entities are dominant (more than 50%) in a pattern." ;
                            rdfs:label "hasDominantPatternEntities"@IRI-based; 
                            rdfs:label "has dominant pattern entities"@en; 
                            rdfs:domain :Pattern;
                            rdfs:range :PatternEntities . 
#  --------------------------- Property 42------------------------- 
:MQIHorizontalJointsVert rdf:type owl:DatatypeProperty ;
                         rdfs:comment "Defines the adequacy of horizontal joints (based on level of horizontality/continuity), in the context of vertical loading." ;
                         rdfs:label "MQIHorizontalJointsVert"@IRI-based; 
                         rdfs:label "MQI-Vertical-Horizontal Joints"@en; 
                         rdfs:domain :MasonryQualityIndex;
                         rdfs:range xsd:float . 
#  --------------------------- Property 43------------------------- 
:MQIMortarQualityVert rdf:type owl:DatatypeProperty ;
                      rdfs:comment "Defines the adequacy of the mortar, in the context of vertical loading." ;
                      rdfs:label "MQIMortarQualityVert"@IRI-based; 
                      rdfs:label "MQI-Vertical-Mortar Quality"@en; 
                      rdfs:domain :MasonryQualityIndex;
                      rdfs:range xsd:float . 
#  --------------------------- Property 44------------------------- 
:isMasonryLayerOf rdf:type owl:ObjectProperty; 
                  owl:inverseOf :hasMasonryLayer ;
                  rdfs:comment "Defines the relationship between a masonry wall and a masonry layer." ;
                  rdfs:label "isMasonryLayerOf"@IRI-based; 
                  rdfs:label "is layer of"@en; 
                  rdfs:domain :MasonryLayer;
                  rdfs:range :MasonryElement . 
#  --------------------------- Property 45------------------------- 
:hasMasonryLayer rdf:type owl:ObjectProperty; 
                 owl:inverseOf :isMasonryLayerOf ;
                 rdfs:comment "Defines the relationship between a masonry wall and a masonry layer." ;
                 rdfs:label "hasMasonryLayer"@IRI-based; 
                 rdfs:label "has layer"@en; 
                 rdfs:domain :MasonryElement;
                 rdfs:range :MasonryLayer . 
#  --------------------------- Property 46------------------------- 
#<https://w3id.org/dot/hasDamageArea> rdf:type owl:ObjectProperty ;
#                                     rdfs:label "hasDamageArea"@IRI-based; 
#                                     rdfs:domain :PatternEntities;
#                                     rdfs:range <https://w3id.org/dot#DamageArea> . 
#  --------------------------- Property 47------------------------- 
:hasMasonryQualityIndex rdf:type owl:ObjectProperty ;
                        rdfs:comment "Defines the Masonry Quality Index associated with a wall" ;
                        rdfs:label "hasMasonryQualityIndex"@IRI-based; 
                        rdfs:label "has Masonry Quality Index"@en; 
                        rdfs:domain :MasonryElement;
                        rdfs:range :MasonryQualityIndex . 
###  Class Definitions (Number of Classes) 24 ###
#  --------------------------- Class  0------------------------- 
#<https://pi.pauwel.be/voc/buildingelement#Wall> rdf:type owl:Class; 
#                                                rdfs:label "Wall"@IRI-based . 
#  --------------------------- Class  1------------------------- 
:TensileStrength rdf:type owl:Class; 
                 rdfs:comment "The average resistance of the homogenised material to breaking under tension." ;
                 owl:disjointWith :MassDensity ;
                 owl:disjointWith :YoungModulus ;
                 rdfs:subClassOf :HomogenisedMechanicalProperty ;
                 rdfs:label "TensileStrength"@IRI-based; 
                 rdfs:label "Tensile Strength"@en . 
#  --------------------------- Class  2------------------------- 
:MassDensity rdf:type owl:Class; 
             rdfs:comment "The mass per unit volume of a masonry wall." ;
             owl:disjointWith :YoungModulus ;
             rdfs:subClassOf :HomogenisedMechanicalProperty ;
             rdfs:label "MassDensity"@IRI-based; 
             rdfs:label "Mass Density"@en . 
#  --------------------------- Class  3------------------------- 
:MasonryLayer rdf:type owl:Class; 
              rdfs:comment "A layer of a masonry wall." ;
              owl:disjointWith :PatternEntities ;
              rdfs:label "MasonryLayer"@IRI-based; 
              rdfs:label "Masonry Layer"@en . 
#  --------------------------- Class  4------------------------- 
#<http://purl.org/vocommons/voaf#Vocabulary> rdf:type owl:Class; 
#                                            rdfs:label "Vocabulary"@IRI-based . 
#  --------------------------- Class  5------------------------- 
#foaf:Person rdf:type owl:Class; 
#            rdfs:label "Person"@IRI-based . 
#  --------------------------- Class  6------------------------- 
#<http://bimerr.iot.linkeddata.es/def/material-properties#Property> rdf:type owl:Class; 
#                                                                   rdfs:label "Property"@IRI-based . 
#  --------------------------- Class  7------------------------- 
:Pattern rdf:type owl:Class; 
         rdfs:comment "The pattern formed by units and joints in a masonry layer." ;
         owl:disjointWith :MasonryLayer ;
         owl:disjointWith :PatternEntities ;
         owl:disjointWith :RepresentativeVolumeElement ;
         rdfs:label "Pattern"@IRI-based; 
         rdfs:label "Pattern"@en . 
#  --------------------------- Class  8------------------------- 
#<https://w3id.org/dot#DamageArea> rdf:type owl:Class; 
#                                  rdfs:comment "imported from https://w3id.org/dot ; used to describe damage in hmo:PatternEntities" ;
#                                  rdfs:label "DamageArea"@IRI-based; 
#                                  rdfs:label "Damage Area"@en . 
#  --------------------------- Class  9------------------------- 
:Units rdf:type owl:Class; 
       rdfs:comment "The configuration of the units in the pattern." ;
       owl:disjointWith :Joints ;
       rdfs:subClassOf :PatternEntities ;
       rdfs:label "Units"@IRI-based; 
       rdfs:label "Units"@en . 
#  --------------------------- Class  10------------------------- 
:YoungModulus rdf:type owl:Class; 
              rdfs:comment "Modulus of longitudinal elasticity." ;
              rdfs:subClassOf :HomogenisedMechanicalProperty ;
              rdfs:label "YoungModulus"@IRI-based; 
              rdfs:label "Young Modulus"@en . 
#  --------------------------- Class  11------------------------- 
:HomogenisedMechanicalProperty rdf:type owl:Class; 
                               rdfs:comment "A mechanical property associated to an entire masonry wall, considering the assembly of units and joints." ;
                               owl:disjointWith :MasonryQualityIndex ;
                               owl:disjointWith :PatternEntities ;
                               owl:disjointWith :Units ;
                               owl:disjointWith :MasonryLayer ;
                               owl:disjointWith :MasonryElement ;
                               owl:disjointWith :Pattern ;
                               owl:disjointWith :RepresentativeVolumeElement ;
                               rdfs:label "HomogenisedMechanicalProperty"@IRI-based; 
                               rdfs:label "Homogenised Mechanical Property"@en . 
#  --------------------------- Class  12------------------------- 
:MortarJoints rdf:type owl:Class; 
              rdfs:comment "Joints made of mortar." ;
              rdfs:subClassOf :Joints ;
              rdfs:label "MortarJoints"@IRI-based; 
              rdfs:label "Mortar Joints"@en . 
#  --------------------------- Class  13------------------------- 
:RepresentativeVolumeElement rdf:type owl:Class; 
#                             owl:equivalentClass <http://bimerr.iot.linkeddata.es/def/material-properties#Material> ;
                             rdfs:comment "In the context of global macro-models, a masonry area to which homogeneous mechanical characteristics can be attributed." ;
                             owl:disjointWith :MasonryLayer ;
                             rdfs:label "RepresentativeVolumeElement"@IRI-based; 
                             rdfs:label "Representative Volume Element"@en . 
#  --------------------------- Class  14------------------------- 
:HorizontalJoints rdf:type owl:Class; 
                  rdfs:comment "Horizontal spaces between masonry units. Can be either dry or made of mortar." ;
                  owl:disjointWith :VerticalJoints ;
                  rdfs:subClassOf :Joints ;
                  rdfs:label "HorizontalJoints"@IRI-based; 
                  rdfs:label "Horizontal Joints"@en . 
#  --------------------------- Class  15------------------------- 
:ShearStrengthTC rdf:type owl:Class; 
                 rdfs:comment "Average shear strength according to the Turnsek and Cacovic criterion. It is used in the case of irregular-textured masonry and corresponds to diagonal tensile failure at the masonry level." ;
                 owl:disjointWith :TensileStrength ;
                 owl:disjointWith :ShearStrengthMC ;
                 owl:disjointWith :CompressiveStrength ;
                 owl:disjointWith :YoungModulus ;
                 owl:disjointWith :MassDensity ;
                 owl:disjointWith :ShearModulus ;
                 rdfs:subClassOf :HomogenisedMechanicalProperty ;
                 rdfs:label "ShearStrengthTC"@IRI-based; 
                 rdfs:label "Shear Strength (Turnsek and Cacovic)"@en . 
#  --------------------------- Class  16------------------------- 
:ShearModulus rdf:type owl:Class; 
              rdfs:comment "Modulus of tangential elasticity." ;
              owl:disjointWith :YoungModulus ;
              owl:disjointWith :TensileStrength ;
              owl:disjointWith :ShearStrengthMC ;
              owl:disjointWith :MassDensity ;
              rdfs:subClassOf :HomogenisedMechanicalProperty ;
              rdfs:label "ShearModulus"@IRI-based; 
              rdfs:label "Shear Modulus"@en . 
#  --------------------------- Class  17------------------------- 
:CompressiveStrength rdf:type owl:Class; 
                     rdfs:comment "The average resistance of the homogenised material to breaking under compression." ;
                     owl:disjointWith :TensileStrength ;
                     owl:disjointWith :ShearStrengthMC ;
                     owl:disjointWith :YoungModulus ;
                     owl:disjointWith :MassDensity ;
                     owl:disjointWith :ShearModulus ;
                     rdfs:subClassOf :HomogenisedMechanicalProperty ;
                     rdfs:label "CompressiveStrength"@IRI-based; 
                     rdfs:label "Compressive Strength"@en . 
#  --------------------------- Class  18------------------------- 
:VerticalJoints rdf:type owl:Class; 
                rdfs:comment "Vertical spaces between masonry units. Can be either dry or made of mortar." ;
                rdfs:subClassOf :Joints ;
                rdfs:label "VerticalJoints"@IRI-based; 
                rdfs:label "Vertical Joints"@en . 
#  --------------------------- Class  19------------------------- 
:PatternEntities rdf:type owl:Class; 
                 rdfs:comment "A group of entities in a pattern which have the same function, geometry and material properties." ;
                 rdfs:label "PatternEntities"@IRI-based; 
                 rdfs:label "Pattern Entities"@en . 
#  --------------------------- Class  20------------------------- 
:MasonryQualityIndex rdf:type owl:Class; 
                     rdfs:comment "A visual method for assessing the structural behavior of masonry walls." ;
                     owl:disjointWith :MasonryElement ;
                     owl:disjointWith :Pattern ;
                     owl:disjointWith :MasonryLayer ;
                     owl:disjointWith :PatternEntities ;
                     owl:disjointWith :RepresentativeVolumeElement ;
                     rdfs:subClassOf :HomogenisedMechanicalProperty ;
                     rdfs:label "MasonryQualityIndex"@IRI-based; 
                     rdfs:label "Masonry Quality Index"@en . 
#  --------------------------- Class  21------------------------- 
:Joints rdf:type owl:Class; 
        rdfs:comment "The configuration of the joints in the pattern." ;
        rdfs:subClassOf :PatternEntities ;
        rdfs:label "Joints"@IRI-based; 
        rdfs:label "Joints"@en . 
#  --------------------------- Class  22------------------------- 
:MasonryElement rdf:type owl:Class; 
             rdfs:comment "A load bearing wall made of structural masorny." ;
             owl:disjointWith :PatternEntities ;
             owl:disjointWith :MasonryLayer ;
             owl:disjointWith :Pattern ;
             rdfs:label "MasonryElement"@IRI-based; 
             rdfs:label "Masonry Element"@en . 
#  --------------------------- Class  23------------------------- 
:ShearStrengthMC rdf:type owl:Class; 
                 rdfs:comment "Average shear strength according to the Mohr-Coulomb criterion. It is used in the case of regular-textured masonry and corresponds to diagonal tensile failure at the joints level." ;
                 owl:disjointWith :YoungModulus ;
                 owl:disjointWith :TensileStrength ;
                 owl:disjointWith :MassDensity ;
                 rdfs:subClassOf :HomogenisedMechanicalProperty ;
                 rdfs:label "ShearStrengthMC"@IRI-based; 
                 rdfs:label "Shear Strength (Mohr Coulomb)"@en . 
